PlutusCore/Cbor/Lemmas.lean
@@ -2,39 +2,43 @@ import PlutusCore.Cbor.Basic
 
 open PlutusCore.Cbor.CborInternal
 
+-- ==============
+-- =  Encoding  =
+-- ==============
+
 example : e₈ 7234295460216005990 = "deadbeef".toList := rfl
 
-example : splitToChunks "" = [] := by simp [splitToChunks]
+example : splitToChunks "" = [] := by native_decide
 
 example : splitToChunks "1234567890123456789012345678901234567890123456789012345678901234" =
-  [ "1234567890123456789012345678901234567890123456789012345678901234" ] := by simp [splitToChunks]
+  [ "1234567890123456789012345678901234567890123456789012345678901234" ] := by native_decide
 
 example : splitToChunks  "12345678901234567890123456789012345678901234567890123456789012345" =
   [ "1234567890123456789012345678901234567890123456789012345678901234"
   , "5"
-  ] := by simp [splitToChunks]
+  ] := by native_decide
 
 example : splitToChunks "1234567890123456789012345678901234567890123456789012345678901234123456789012345678901234567890123456789012345678901234567890123456" =
   [ "1234567890123456789012345678901234567890123456789012345678901234"
   , "1234567890123456789012345678901234567890123456789012345678901234"
   , "56"
-  ] := by simp [splitToChunks]
+  ] := by native_decide
 
 example : encodeBytestring "1234567890123456789012345678901234567890123456789012345678901234" =
-  .some ("\x58\x40" ++ "1234567890123456789012345678901234567890123456789012345678901234") := by simp [encodeBytestring, splitToChunks, encodeBytestringChunk, encodeHead]
+  .some ("\x58\x40" ++ "1234567890123456789012345678901234567890123456789012345678901234") := by native_decide
 
 example : encodeBytestring "12345678901234567890123456789012345678901234567890123456789012345" =
   .some ("\x5F"
          ++ "\x58\x40" ++ "1234567890123456789012345678901234567890123456789012345678901234"
          ++ "\x41"     ++ "5"
-         ++ "\xFF") := by simp [encodeBytestring, splitToChunks, encodeBytestringChunk, encodeHead, encodeIndef]
+         ++ "\xFF") := by native_decide
 
 example : encodeBytestring "1234567890123456789012345678901234567890123456789012345678901234123456789012345678901234567890123456789012345678901234567890123456" =
   .some ("\x5F"
          ++ "\x58\x40" ++ "1234567890123456789012345678901234567890123456789012345678901234"
          ++ "\x58\x40" ++ "1234567890123456789012345678901234567890123456789012345678901234"
          ++ "\x42"     ++ "56"
-         ++ "\xFF") := by simp [encodeBytestring, splitToChunks, encodeBytestringChunk, encodeHead, encodeIndef]
+         ++ "\xFF") := by native_decide
 
 example : encodeData (.I 12) = .some "\x0c"     := by simp [encodeData, encodeInt, encodeHead]
 example : encodeData (.I 42) = .some "\x18\x2a" := by simp [encodeData, encodeInt, encodeHead]
@@ -45,8 +49,7 @@ example :
         .Constr 0 [.I 1284531],
         .I 1739713998000
       ]
-    ) = .some "\xd8\x79\x9f\xd8\x79\x9f\x1a\x00\x13\x99\xb3\xff\x1b\x00\x00\x01\x95\x0f\x08\xec\xb0\xff" := by
-          simp [encodeData, encodeCtag, encodeHead, encodeInt, encodeIndef, String.singleton, Char.ofNat, Nat.isValidChar, String.push]
+    ) = .some "\xd8\x79\x9f\xd8\x79\x9f\x1a\x00\x13\x99\xb3\xff\x1b\x00\x00\x01\x95\x0f\x08\xec\xb0\xff" := by native_decide
 
 example :
   encodeData (
@@ -55,5 +58,36 @@ example :
       .I 22710,
       .I 4387720097
     ]
-  ) = .some "\xd8\x79\x9f\x1a\x08\x9a\xfe\x76\x19\x58\xb6\x1b\x00\x00\x00\x01\x05\x87\x4b\xa1\xff" := by
-          simp [encodeData, encodeCtag, encodeHead, encodeInt, encodeIndef, String.singleton, Char.ofNat, Nat.isValidChar, String.push]
+  ) = .some "\xd8\x79\x9f\x1a\x08\x9a\xfe\x76\x19\x58\xb6\x1b\x00\x00\x00\x01\x05\x87\x4b\xa1\xff" := by native_decide
+
+-- ==============
+-- =  Decoding  =
+-- ==============
+
+example : d₈ "deadbeef".toList = .some ([], 7234295460216005990) := by rfl
+example : d₁ "deadbeef".toList = .some ("eadbeef".toList, 100)   := by rfl
+
+example : decodeBytestring ("\x58\x40" ++ "1234567890123456789012345678901234567890123456789012345678901234") =
+  .some ("", "1234567890123456789012345678901234567890123456789012345678901234") := by native_decide
+
+example : decodeData "\x0C"     = .some ("", .I 12) := by native_decide
+example : decodeData "\x18\x2A" = .some ("", .I 42) := by native_decide
+
+example : decodeData "\xd8\x79\x9f\xd8\x79\x9f\x1a\x00\x13\x99\xb3\xff\x1b\x00\x00\x01\x95\x0f\x08\xec\xb0\xff\x34\x32"
+    = .some (
+        "42",
+        .Constr 0 [
+          .Constr 0 [.I 1284531],
+          .I 1739713998000
+        ]
+      ) := by native_decide
+
+example : decodeData "\xd8\x79\x9f\x1a\x08\x9a\xfe\x76\x19\x58\xb6\x1b\x00\x00\x00\x01\x05\x87\x4b\xa1\xff\x43\x62\x6f\x72\x44\x61\x74\x61"
+  = .some (
+      "CborData",
+      .Constr 0 [
+        .I 144375414,
+        .I 22710,
+        .I 4387720097
+      ]
+  ) := by native_decide
